comment on the Coq code and generate documentation in HTML

language_formal/spark2014_semantics/environment.v
@@ -1,20 +1,11 @@
-Require Export language.
 Require Export values.
 
-(*
-    stack  /-----------------------------
-              |- stack data structure
-              | -----------------------------
-              |- stack operations
-              | -----------------------------
-              |- stack lemmas
-              | -----------------------------
-*)
+(** * Stack *)
 
-(* # stack as a list *)
+(** ** Stack as a list *)
 Definition stack : Type := list (idnum * val).
 
-(* # stack operations *)
+(** ** Stack operations *)
 Function reside (x : idnum) (s : stack) := 
     match s with 
     | (y, v) :: s' =>
@@ -25,7 +16,7 @@ Function reside (x : idnum) (s : stack) :=
     | nil => false
     end.
 
-(* fetch the value of x that has already been initialized in stack *)
+(** fetch the value of x that has already been initialized in stack *)
 Function fetch (x : idnum) (s : stack): option value := 
     match s with 
     | (y, v) :: s' =>
@@ -38,7 +29,7 @@ Function fetch (x : idnum) (s : stack): option value :=
     | nil => None
     end.
 
-(* update the latest binding for x *)
+(** update the latest binding for x *)
 Function update (s: stack) (x : idnum) (v: val): option stack := 
     match s with 
     | (y, v') :: s' => 
@@ -52,13 +43,7 @@ Function update (s: stack) (x : idnum) (v: val): option stack :=
    | nil => None
    end.
 
-(*
-Lemma update_fetch_new: forall s x v s',
-    update s x v = Some s' ->
-    fetch x s' = Some v.
-*)
-
-(* # lemmas about stack operations *)
+(** ** Lemmas about stack operations *)
 Lemma fetch_in: forall x s v, fetch x s = Some v -> List.In (x, Value v) s.
 Proof.
     intros x s.
@@ -80,7 +65,7 @@ Proof.
     inversion H.
 Qed.
 
-Lemma update_in: forall s x v' s', Some s' = update s x v' -> (exists v, List.In (x, v) s).
+Lemma update_in: forall s x v' s', update s x v' = Some s' -> (exists v, List.In (x, v) s).
 Proof.
     intros s x v'.
     functional induction (update s x v');
@@ -89,8 +74,7 @@ Proof.
     end; intros s1 h1.
   - exists v'. 
     simpl. left; auto.
-  - symmetry in e1.
-    specialize (IHo s'' e1).
+  - specialize (IHo s'' e1).
     inversion IHo.
     exists x0. simpl. 
     right; assumption.
@@ -99,7 +83,7 @@ Proof.
 Qed.
     
 Lemma in_update: forall s x v' y v s',
-                   Some s' = update s x v' ->
+                   update s x v' = Some s' ->
                    List.In (y, v) s'
                    -> ((y=x /\ v=v') \/ List.In (y,v) s).
 Proof.
@@ -110,8 +94,7 @@ Proof.
   - destruct h'.
     + left. inversion H; auto.
     + right. right; assumption.
-  - symmetry in e1.
-    specialize (IHo y0 v0 s'' e1).
+  - specialize (IHo y0 v0 s'' e1).
     destruct h'.
     + right. left. assumption.
     + specialize (IHo H). 
@@ -120,43 +103,144 @@ Proof.
        * right. right; assumption.
 Qed.
 
-(* - - - - - - - - - - - - - - - - - - - - - - - - - - - - - - - - - - - - - - - - - - - - - - - - *)
-(* - - - - - - - - - - - - - - - - - - - - - - - - - - - - - - - - - - - - - - - - - - - - - - - - *)
+(** * Symbol Table *)
 
-(*
-    symbol_table  /-----------------------------
-                           |- symtb data structure
-                           | -----------------------------
-                           |- symtb operations
-                           | -----------------------------
-                           |- symtb lemmas (to be added)
-                           | -----------------------------
-*)
-
-(* # symbol table: var -> (mode * type) *)
+(** ** Symbol table as a list *)
 Definition symtb: Type := list (idnum * (mode * typ)).
 
+(** ** Symbol table operations *)
 Fixpoint lookup (x : idnum) (tb: symtb) := 
    match tb with 
    | (y, (m,t)) :: tb' => if (beq_nat x y) then Some (m, t) else lookup x tb' 
    | nil => None
    end.
 
-(* - - - - - - - - - - - - - - - - - - - - - - - - - - - - - - - - - - - - - - - - - - - - - - - - *)
-(* - - - - - - - - - - - - - - - - - - - - - - - - - - - - - - - - - - - - - - - - - - - - - - - - *)
-
-(* 
+(** * Program State *)
+(** 
     possible state after running a command:
-    - (1) a normal resultant stack
-    - (2) undefined variables (in expression or assigned to an undefined variable), 
-            uninitialized variables, type checking failure
-    - (3) a security constraint is violated (overflow, division by zero)
+    - a normal resultant stack
+    - an exception (such as overflow, division by zero and so on)
+    - an unterminated state
 *)
 Inductive state: Type :=
     | SNormal: stack -> state
     | SException: state
     | SUnterminated: state.
 (*    | SAbnormal: state (* for state (1) above *) *)
+
+(** * Type Check Stack *)
+
+(** ** Type checker *)
+Inductive type_check_stack: symtb -> stack -> Prop :=
+    | TC_Empty: type_check_stack nil nil
+    | TC_Bool: forall tb s x m b,
+          type_check_stack tb s ->
+          type_check_stack ((x, (m, Tbool)) :: tb) ((x, (Value (Bool b))) :: s)
+    | TC_Int: forall tb s x m v,
+          type_check_stack tb s ->
+          type_check_stack ((x, (m, Tint)) :: tb) ((x, (Value (Int v))) :: s)
+    | TC_UndefBool: forall tb s x m,
+          type_check_stack tb s ->
+          type_check_stack ((x, (m, Tbool)) :: tb) ((x, Vundef) :: s)
+    | TC_UndefInt: forall tb s x m,
+          type_check_stack tb s ->
+          type_check_stack ((x, (m, Tint)) :: tb) ((x, Vundef) :: s).
+
+(*
+Inductive symbol_consistent: stack -> symtb -> Prop :=
+    | SymCons: forall (s: stack) (tb: symtb), 
+        ( forall x v, Some v = fetch x s -> 
+                          (exists t, stored_value_type (Value v) t /\ ( exists m, lookup x tb = Some (m, t)))) -> 
+        (forall x m t, lookup x tb = Some (m, t) -> 
+                          reside x s = true /\ 
+                          (forall v, (Some v = fetch x s) -> stored_value_type (Value v) t)) -> 
+        symbol_consistent s tb.
+*)
+
+(** ** Some lemmas *)
+Lemma typed_value: forall tb s x v,
+    type_check_stack tb s ->
+    fetch x s = Some v ->
+    (exists t, stored_value_type (Value v) t /\ ( exists m, lookup x tb = Some (m, t))).
+Proof.
+    intros tb s x v h1 h2.
+    destruct v.
+  - exists Tint.
+    split.
+    + constructor.
+    + induction h1;
+       [inversion h2 | | | | ];
+       unfold fetch in h2;
+       unfold lookup;
+       destruct (beq_nat x x0);
+       [ inversion h2 | | exists m; auto | | inversion h2 | | inversion h2 | ];
+       fold fetch in h2;
+       fold lookup;
+       specialize (IHh1 h2);
+       assumption.
+  - exists Tbool.
+    split.
+    + constructor.
+    + induction h1;
+       [inversion h2 | | | | ];
+       unfold fetch in h2;
+       unfold lookup;
+       destruct (beq_nat x x0);
+       [ exists m; auto | | inversion h2 | | inversion h2 | | inversion h2 | ];
+       fold fetch in h2;
+       fold lookup;
+       specialize (IHh1 h2);
+       assumption.
+Qed.
+
+Ltac rm_exists1 :=
+    repeat match goal with
+    | [ h: exists _, _ |- _ ] => inversion h; clear h
+    | [ h: _ /\ _  |- _ ] => inversion h; clear h
+    end.
+
+Ltac tv_l1 f1 f2 h1 h2 x x0 := 
+    unfold f1 in h1;
+    unfold f2;
+    destruct (beq_nat x x0);
+    [ auto |
+      fold f1 in h1;
+      fold f2;
+      specialize (h2 h1);
+      rm_exists1; auto
+    ].
+
+Ltac tv_l2 f1 f2 h1 h2 x x0 tac :=
+    unfold f1 in h1;
+    unfold f2;
+    destruct (beq_nat x x0);
+    [ intros; 
+      inversion h1; subst;
+      inversion H; subst; 
+      tac |
+      fold f1 in h1;
+      fold f2;
+      specialize (h2 h1);
+      rm_exists1; auto
+    ].
+
+Lemma typed_value': forall tb s x m t,
+    type_check_stack tb s ->
+    lookup x tb = Some (m, t) -> 
+    reside x s = true /\ 
+    (forall v, (Some v = fetch x s) -> stored_value_type (Value v) t).
+Proof.
+    intros tb s x m t h1 h2.
+    induction h1;
+    [inversion h2 | | | | ];
+    split;
+    [ | tv_l2 lookup fetch h2 IHh1 x x0 constructor |
+      | tv_l2 lookup fetch h2 IHh1 x x0 constructor |
+      | tv_l2 lookup fetch h2 IHh1 x x0 auto |
+      | tv_l2 lookup fetch h2 IHh1 x x0 auto
+    ];
+    tv_l1 lookup reside h2 IHh1 x x0.
+Qed.
 
 
 
